proof/agp32_MEM_Data_CorrectScript.sml
@@ -1,10 +1,82 @@
-open hardwarePreamble translatorTheory translatorLib arithmeticTheory pred_setTheory wordsExtraTheory dep_rewrite blastLib bitstringSyntax fcpSyntax listSyntax wordsSyntax agp32StateTheory agp32EnvironmentTheory agp32ProcessorTheory ag32Theory ag32ExtraTheory ag32UtilitiesTheory agp32RelationTheory agp32UpdateTheory agp32InternalTheory agp32StepLib agp32_MEM_CorrectTheory;
+open hardwarePreamble translatorTheory translatorLib arithmeticTheory pred_setTheory wordsExtraTheory dep_rewrite blastLib bitstringSyntax fcpSyntax listSyntax wordsSyntax agp32StateTheory agp32EnvironmentTheory agp32ProcessorTheory ag32Theory ag32ExtraTheory ag32UtilitiesTheory agp32RelationTheory agp32UpdateTheory agp32InternalTheory agp32SpecialTheory agp32StepLib agp32_MEM_CorrectTheory;
 
 (* correctness of memory and data loading with respect to the ISA *)
 val _ = new_theory "agp32_MEM_Data_Correct";
 
 val _ = prefer_num ();
 val _ = guess_lengths ();
+
+
+(** lemma **)
+Theorem WB_opc_unchanged_after_disabled_cycles[local]:
+  !fext fbits m n.
+    (!p. p < m ==> ~(fext (p + n)).ready) ==>
+    (agp32 fext fbits (m + n)).WB.WB_opc = (agp32 fext fbits n).WB.WB_opc
+Proof
+  rw [] >> Induct_on `m` >> rw [] >>
+  `!p. p < m ==> ~(fext (n + p)).ready` by fs [] >> fs [] >>
+  `m < SUC m` by rw [] >>
+  `~(fext (n + m)).ready` by fs [] >>
+  `~(agp32 fext fbits (n + m)).WB.WB_state_flag`
+    by METIS_TAC [agp32_WB_state_flag_and_fext_ready] >>
+  `(agp32 fext fbits (SUC (n + m))).WB.WB_opc = (agp32 fext fbits (n + m)).WB.WB_opc`
+    by fs [agp32_WB_opc_unchanged_when_WB_disabled,enable_stg_def] >>
+  `n + SUC m = SUC (n + m)` by rw [] >> rw [] >> fs []
+QED
+
+Theorem data_addr_wdata_wstrb_unchanged_after_disabled_cycles[local]:
+  !fext fbits m n.
+    (!p. p < m ==> ~(fext (p + n)).ready) ==>
+    ((agp32 fext fbits (m + n)).data_addr = (agp32 fext fbits n).data_addr) /\
+    ((agp32 fext fbits (m + n)).data_wdata = (agp32 fext fbits n).data_wdata) /\
+    ((agp32 fext fbits (m + n)).data_wstrb = (agp32 fext fbits n).data_wstrb)
+Proof
+  rw [] >> Induct_on `m` >> rw [] >>
+  `!p. p < m ==> ~(fext (n + p)).ready` by fs [] >> fs [] >>
+  `m < SUC m` by rw [] >>
+  `~(fext (n + m)).ready` by fs [] >>
+  `~(agp32 fext fbits (n + m)).WB.WB_state_flag`
+    by METIS_TAC [agp32_WB_state_flag_and_fext_ready] >>
+  `(agp32 fext fbits (SUC (n + m))).data_addr = (agp32 fext fbits (n + m)).data_addr /\
+  (agp32 fext fbits (SUC (n + m))).data_wdata = (agp32 fext fbits (n + m)).data_wdata /\
+  (agp32 fext fbits (SUC (n + m))).data_wstrb = (agp32 fext fbits (n + m)).data_wstrb`
+    by fs [agp32_data_addr_wstrb_wdata_unchanged_when_WB_disabled,enable_stg_def] >>
+  `n + SUC m = SUC (n + m)` by rw [] >> rw [] >> fs []
+QED
+
+Theorem WB_opc_unchanged_after_disabled_cycles_0[local]:
+  !fext fbits m.
+    (!p. p < m ==> ~(fext p).ready) ==>
+    (agp32 fext fbits m).WB.WB_opc = (agp32 fext fbits 0).WB.WB_opc
+Proof
+  rw [] >> `!p. p < m ==> ~(fext (p + 0)).ready` by fs [] >>
+  `(agp32 fext fbits (m + 0)).WB.WB_opc = (agp32 fext fbits 0).WB.WB_opc`
+    by fs [WB_opc_unchanged_after_disabled_cycles] >> fs []
+QED
+
+Theorem EMPTY_no_fext_ready_cycle[local]:
+  !t fext.
+    {t0 | t0 < t /\ (fext t0).ready} = {} ==>
+    (!t0. t0 < t ==> ~(fext t0).ready)
+Proof
+  rw [] >> Cases_on `(fext t0).ready` >> rw [] >>
+  `t0 IN {t0 | t0 < t /\ (fext t0).ready}` by fs [] >>
+  METIS_TAC [MEMBER_NOT_EMPTY]
+QED
+
+Theorem MAX_SET_0_no_fext_ready_cycle[local]:
+  !t fext.
+    {t0 | t0 < t /\ (fext t0).ready} <> {} ==>
+    MAX_SET {t0 | t0 < t /\ (fext t0).ready} = 0 ==>
+    (!t0. t0 < t - 1 ==> ~(fext (t0 + 1)).ready)
+Proof
+  rw [] >>
+  `FINITE {t0 | t0 < t /\ (fext t0).ready}` by rw [FINITE_max_ready_cycle] >>
+  Cases_on `(fext (t0 + 1)).ready` >> rw [] >>
+  `t0 + 1  < t` by fs [] >>
+  `t0 + 1 IN {t0 | t0 < t /\ (fext t0).ready}` by fs [] >>
+  `t0 + 1 <= 0` by METIS_TAC [MAX_SET_DEF] >> rw []
+QED
 
 
 (** memory **)
@@ -49,23 +121,58 @@ Proof
         `~(fext (0 + SUC t)).ready` by fs [] >> fs []) >>
       last_assum (mp_tac o is_mem_do_nothing `SUC t`) >> rw [] >>
       `THE (I' (4,t)) = THE (I' (5,t)) + 1`
-        by METIS_TAC [MEM_instr_index_with_WB_instr_plus_1] >> fs [Rel_def]) >> fs [] >>
+        by METIS_TAC [MEM_instr_index_with_WB_instr_plus_1] >> fs [Rel_def]) >>
     fs [is_wrMEM_isa_def] >-
      (`(agp32 fext fbits t).MEM.MEM_opc = 2w` by fs [is_wrMEM_isa_def,Rel_def,MEM_Rel_def] >>
+      `(agp32 fext fbits (SUC t)).WB.WB_opc = 2w` by fs [agp32_WB_opc_MEM_opc_when_WB_enabled] >>
       `(agp32 fext fbits (SUC t)).command = 3w`
-        by fs [agp32_Rel_ag32_command_correct_write_mem_WB_enable,
-               agp32_WB_opc_MEM_opc_when_WB_enabled] >>
+        by fs [agp32_Rel_ag32_command_correct_write_mem_WB_enable] >>
+      `align_addr (agp32 fext fbits (SUC t)).data_addr =
+      mem_data_addr (FUNPOW Next (THE (I' (4,t)) − 1) a)`
+        by METIS_TAC [agp32_Rel_ag32_data_addr_correct_write_mem] >>
+      `(agp32 fext fbits (SUC t)).data_wdata =
+      mem_data_wdata (FUNPOW Next (THE (I' (4,t)) − 1) a)`
+        by METIS_TAC [agp32_Rel_ag32_data_wdata_correct_write_mem] >>
+      `(agp32 fext fbits (SUC t)).data_wstrb =
+      mem_data_wstrb (FUNPOW Next (THE (I' (4,t)) − 1) a)`
+        by METIS_TAC [agp32_Rel_ag32_data_wstrb_correct_write_mem] >>
       last_assum (mp_tac o is_mem_data_write `SUC t`) >> rw [] >>
       Cases_on `m` >> fs [] >-
-       (cheat) >>
+       (`THE (I' (4,t)) = SUC (THE (I' (5,t)))`
+          by METIS_TAC [MEM_instr_index_with_WB_instr_plus_1,ADD1] >> fs [FUNPOW_SUC] >>
+        qpat_abbrev_tac `ai = FUNPOW Next _ a` >>
+        fs [ag32_StoreMEM_mem_update,Rel_def]) >>
       `~(fext (0 + SUC t)).ready` by fs [] >> fs []) >>
     `(agp32 fext fbits t).MEM.MEM_opc = 3w` by fs [is_wrMEM_isa_def,Rel_def,MEM_Rel_def] >>
+    `(agp32 fext fbits (SUC t)).WB.WB_opc = 3w` by fs [agp32_WB_opc_MEM_opc_when_WB_enabled] >>
     `(agp32 fext fbits (SUC t)).command = 3w`
-      by fs [agp32_Rel_ag32_command_correct_write_mem_byte_WB_enable,
-             agp32_WB_opc_MEM_opc_when_WB_enabled] >>
+      by fs [agp32_Rel_ag32_command_correct_write_mem_byte_WB_enable] >>
+    `(agp32 fext fbits (SUC t)).data_addr = mem_data_addr (FUNPOW Next (THE (I' (4,t)) − 1) a)`
+      by METIS_TAC [agp32_Rel_ag32_data_addr_correct_write_mem_byte] >>
+    `(agp32 fext fbits (SUC t)).data_wstrb = mem_data_wstrb (FUNPOW Next (THE (I' (4,t)) − 1) a)`
+      by METIS_TAC [agp32_Rel_ag32_data_wstrb_correct_write_mem_byte] >>
+    `word_bit 0 (mem_data_wstrb (FUNPOW Next (THE (I' (4,t)) − 1) a)) ==>
+    (7 >< 0) (agp32 fext fbits (SUC t)).data_wdata =
+    mem_data_wdata_byte (FUNPOW Next (THE (I' (4,t)) − 1) a)`
+      by METIS_TAC [agp32_Rel_ag32_data_wdata_correct_write_mem_byte_word_bit_0] >>
+    `word_bit 1 (mem_data_wstrb (FUNPOW Next (THE (I' (4,t)) − 1) a)) ==>
+    (15 >< 8) (agp32 fext fbits (SUC t)).data_wdata =
+    mem_data_wdata_byte (FUNPOW Next (THE (I' (4,t)) − 1) a)`
+      by METIS_TAC [agp32_Rel_ag32_data_wdata_correct_write_mem_byte_word_bit_1] >>
+    `word_bit 2 (mem_data_wstrb (FUNPOW Next (THE (I' (4,t)) − 1) a)) ==>
+    (23 >< 16) (agp32 fext fbits (SUC t)).data_wdata =
+    mem_data_wdata_byte (FUNPOW Next (THE (I' (4,t)) − 1) a)`
+      by METIS_TAC [agp32_Rel_ag32_data_wdata_correct_write_mem_byte_word_bit_2] >>
+    `word_bit 3 (mem_data_wstrb (FUNPOW Next (THE (I' (4,t)) − 1) a)) ==>
+    (31 >< 24) (agp32 fext fbits (SUC t)).data_wdata =
+    mem_data_wdata_byte (FUNPOW Next (THE (I' (4,t)) − 1) a)`
+      by METIS_TAC [agp32_Rel_ag32_data_wdata_correct_write_mem_byte_word_bit_3] >>
     last_assum (mp_tac o is_mem_data_write `SUC t`) >> rw [] >>
     Cases_on `m` >> fs [] >-
-     (cheat) >>
+     (`THE (I' (4,t)) = SUC (THE (I' (5,t)))`
+        by METIS_TAC [MEM_instr_index_with_WB_instr_plus_1,ADD1] >> fs [FUNPOW_SUC] >>
+      qpat_abbrev_tac `ai = FUNPOW Next _ a` >>
+      fs [ag32_StoreMEMByte_mem_update,Rel_def]) >>
     `~(fext (0 + SUC t)).ready` by fs [] >> fs []) >>
   Cases_on `~is_wrMEM_isa (FUNPOW Next (THE (I' (4,t)) - 1) a)` >-
    (fs [GSYM MEM_not_changed_after_normal_instrs] >>
@@ -88,8 +195,249 @@ Proof
       Cases_on `m` >> fs [] >-
        fs [Rel_def] >>
       `~(fext (0 + SUC t)).ready` by fs [] >> fs []) >>
-    last_assum (mp_tac o is_mem_do_nothing `SUC t`) >> rw [] >> fs [Rel_def]) >> fs [] >>
-  cheat
+    last_assum (mp_tac o is_mem_do_nothing `SUC t`) >> rw [] >> fs [Rel_def]) >>
+  fs [is_wrMEM_isa_def] >-
+   (`(agp32 fext fbits t).MEM.MEM_opc = 2w` by fs [is_wrMEM_isa_def,Rel_def,MEM_Rel_def] >>
+    `(agp32 fext fbits (SUC t)).WB.WB_opc = 2w` by fs [agp32_WB_opc_MEM_opc_when_WB_enabled] >>
+    `(agp32 fext fbits (SUC t)).command = 3w`
+      by fs [agp32_Rel_ag32_command_correct_write_mem_WB_enable] >>
+    `align_addr (agp32 fext fbits (SUC t)).data_addr =
+    mem_data_addr (FUNPOW Next (THE (I' (4,t)) − 1) a)`
+      by METIS_TAC [agp32_Rel_ag32_data_addr_correct_write_mem] >>
+    `(agp32 fext fbits (SUC t)).data_wdata =
+    mem_data_wdata (FUNPOW Next (THE (I' (4,t)) − 1) a)`
+      by METIS_TAC [agp32_Rel_ag32_data_wdata_correct_write_mem] >>
+    `(agp32 fext fbits (SUC t)).data_wstrb =
+    mem_data_wstrb (FUNPOW Next (THE (I' (4,t)) − 1) a)`
+      by METIS_TAC [agp32_Rel_ag32_data_wstrb_correct_write_mem] >>
+    last_assum (mp_tac o is_mem_data_write `SUC t`) >> rw [] >>
+    Cases_on `m` >> fs [] >-
+     (Cases_on `THE (I' (4,t))` >-
+       METIS_TAC [MEM_instr_index_not_0] >> 
+      fs [FUNPOW_SUC] >> qpat_abbrev_tac `ai = FUNPOW Next _ a` >>
+      fs [ag32_StoreMEM_mem_update,Rel_def]) >> 
+    `~(fext (0 + SUC t)).ready` by fs [] >> fs []) >>
+  `(agp32 fext fbits t).MEM.MEM_opc = 3w` by fs [is_wrMEM_isa_def,Rel_def,MEM_Rel_def] >>
+  `(agp32 fext fbits (SUC t)).WB.WB_opc = 3w` by fs [agp32_WB_opc_MEM_opc_when_WB_enabled] >>
+  `(agp32 fext fbits (SUC t)).command = 3w`
+    by fs [agp32_Rel_ag32_command_correct_write_mem_byte_WB_enable] >>
+  `(agp32 fext fbits (SUC t)).data_addr = mem_data_addr (FUNPOW Next (THE (I' (4,t)) − 1) a)`
+    by METIS_TAC [agp32_Rel_ag32_data_addr_correct_write_mem_byte] >>
+  `(agp32 fext fbits (SUC t)).data_wstrb = mem_data_wstrb (FUNPOW Next (THE (I' (4,t)) − 1) a)`
+    by METIS_TAC [agp32_Rel_ag32_data_wstrb_correct_write_mem_byte] >>
+  `word_bit 0 (mem_data_wstrb (FUNPOW Next (THE (I' (4,t)) − 1) a)) ==>
+  (7 >< 0) (agp32 fext fbits (SUC t)).data_wdata =
+  mem_data_wdata_byte (FUNPOW Next (THE (I' (4,t)) − 1) a)`
+    by METIS_TAC [agp32_Rel_ag32_data_wdata_correct_write_mem_byte_word_bit_0] >>
+  `word_bit 1 (mem_data_wstrb (FUNPOW Next (THE (I' (4,t)) − 1) a)) ==>
+  (15 >< 8) (agp32 fext fbits (SUC t)).data_wdata =
+  mem_data_wdata_byte (FUNPOW Next (THE (I' (4,t)) − 1) a)`
+    by METIS_TAC [agp32_Rel_ag32_data_wdata_correct_write_mem_byte_word_bit_1] >>
+  `word_bit 2 (mem_data_wstrb (FUNPOW Next (THE (I' (4,t)) − 1) a)) ==>
+  (23 >< 16) (agp32 fext fbits (SUC t)).data_wdata =
+  mem_data_wdata_byte (FUNPOW Next (THE (I' (4,t)) − 1) a)`
+    by METIS_TAC [agp32_Rel_ag32_data_wdata_correct_write_mem_byte_word_bit_2] >>
+  `word_bit 3 (mem_data_wstrb (FUNPOW Next (THE (I' (4,t)) − 1) a)) ==>
+  (31 >< 24) (agp32 fext fbits (SUC t)).data_wdata =
+  mem_data_wdata_byte (FUNPOW Next (THE (I' (4,t)) − 1) a)`
+    by METIS_TAC [agp32_Rel_ag32_data_wdata_correct_write_mem_byte_word_bit_3] >>
+  last_assum (mp_tac o is_mem_data_write `SUC t`) >> rw [] >>
+  Cases_on `m` >> fs [] >-       
+   (Cases_on `THE (I' (4,t))` >-
+     METIS_TAC [MEM_instr_index_not_0] >>
+    fs [FUNPOW_SUC] >> qpat_abbrev_tac `ai = FUNPOW Next _ a` >>
+    fs [ag32_StoreMEMByte_mem_update,Rel_def]) >>  
+  `~(fext (0 + SUC t)).ready` by fs [] >> fs []
+QED
+
+(** WB disabled and the previous cycle is not ready **)
+Theorem agp32_Rel_ag32_fext_MEM_correct_WB_not_NONE_WB_disable_fext_not_ready:
+  !fext fbits a t I.
+    is_mem fext_accessor_circuit (agp32 fext fbits) fext ==>
+    is_sch I (agp32 fext fbits) a ==>
+    Rel I (fext t) (agp32 fext fbits (t-1)) (agp32 fext fbits t) a t ==>
+    I (5,SUC t) <> NONE ==>
+    (fext (SUC t)).ready ==>
+    ~(fext t).ready ==>
+    ~enable_stg 5 (agp32 fext fbits t) ==>
+    (fext (SUC t)).mem = (FUNPOW Next (THE (I (5,SUC t))) a).MEM
+Proof
+  rw [] >>
+  `(agp32 fext fbits (SUC t)).WB.WB_opc <> 16w` by METIS_TAC [WB_instr_index_not_NONE_opc_not_16] >>
+  Cases_on `MAX_SET {t0 | t0 < t /\ (fext t0).ready}` >-
+   (Cases_on `{t0 | t0 < t /\ (fext t0).ready} = {}` >-
+     (`!t0. t0 < t ==> ~(fext t0).ready` by METIS_TAC [EMPTY_no_fext_ready_cycle] >>
+      `(agp32 fext fbits t).WB.WB_opc = (agp32 fext fbits 0).WB.WB_opc`
+        by fs [WB_opc_unchanged_after_disabled_cycles_0] >>
+      gs [agp32_WB_opc_unchanged_when_WB_disabled,agp32_init_WB_opc]) >>
+    `!t0. t0 < t - 1 ==> ~(fext (t0 + 1)).ready`
+      by METIS_TAC [MAX_SET_0_no_fext_ready_cycle] >>
+    `(agp32 fext fbits (t - 1 + 1)).WB.WB_opc = (agp32 fext fbits 1).WB.WB_opc`
+      by fs [WB_opc_unchanged_after_disabled_cycles] >>
+    `t - 1 + 1 = t` by (Cases_on `t` >> fs []) >> fs [] >>
+    `(agp32 fext fbits t).WB.WB_opc <> 16w` by gs [agp32_WB_opc_unchanged_when_WB_disabled] >>
+    `~enable_stg 5 (agp32 fext fbits 0)` by fs [agp32_init_ctrl_flags,enable_stg_def] >>
+    `(agp32 fext fbits (SUC 0)).WB.WB_opc = 16w`
+      by fs [agp32_WB_opc_unchanged_when_WB_disabled,agp32_init_WB_opc] >>
+    fs [SUC_ONE_ADD]) >>
+  Q.ABBREV_TAC `i = SUC n` >> `i <> 0` by fs [Abbr `i`] >>
+  `FINITE {t0 | t0 < t /\ (fext t0).ready}` by fs [FINITE_max_ready_cycle] >>
+  Cases_on `{t0 | t0 < t /\ (fext t0).ready} = {}` >> fs [MAX_SET_DEF] >>
+  `i IN {t0 | t0 < t /\ (fext t0).ready}` by METIS_TAC [MAX_SET_DEF] >> fs [MAX_SET_DEF] >>
+  last_assum (assume_tac o is_mem_def_mem_no_errors) >>
+  Cases_on_word_value `(agp32 fext fbits (SUC i)).command` >>
+  fs [agp32_command_impossible_values] >-
+   (last_assum (mp_tac o is_mem_data_flush `SUC i`) >> simp [] >> strip_tac >>
+    `m + SUC i = SUC t` by METIS_TAC [same_t_and_m_under_MAX_SET_SUC] >> fs [] >>
+    `I' (5,SUC t) = I' (5,t)` by fs [is_sch_def,is_sch_disable_def] >>
+    `(agp32 fext fbits (SUC i)).WB.WB_opc = (agp32 fext fbits (SUC t)).WB.WB_opc`
+      by METIS_TAC [WB_opc_unchanged_after_disabled_cycles] >>
+    Cases_on `~enable_stg 5 (agp32 fext fbits i)` >-
+     gs [agp32_Rel_ag32_command_correct_WB_disable_fext_ready] >>
+    `(fext i).mem = (fext (m - 1 + SUC i)).mem` by fs [] >>
+    `m - 1 + SUC i = t` by fs [] >> fs [] >>
+    Cases_on `~is_wrMEM_isa (FUNPOW Next (THE (I' (5,t)) - 1) a)` >-
+     fs [GSYM MEM_not_changed_after_normal_instrs,Rel_def] >>
+    fs [is_wrMEM_isa_def] >>
+    `(agp32 fext fbits (SUC t)).WB.WB_opc = (agp32 fext fbits t).WB.WB_opc`
+      by fs [agp32_WB_opc_unchanged_when_WB_disabled] >>
+    fs [Rel_def,WB_Rel_def] >>
+    gs [agp32_Rel_ag32_command_correct_write_mem_WB_enable,
+        agp32_Rel_ag32_command_correct_write_mem_byte_WB_enable]) >-
+   (last_assum (mp_tac o is_mem_data_write `SUC i`) >> simp [] >> strip_tac >>
+    `m + SUC i = SUC t` by METIS_TAC [same_t_and_m_under_MAX_SET_SUC] >> fs [] >>
+    `I' (5,SUC t) = I' (5,t)` by fs [is_sch_def,is_sch_disable_def] >>
+    `(agp32 fext fbits (SUC i)).WB.WB_opc = (agp32 fext fbits (SUC t)).WB.WB_opc`
+      by METIS_TAC [WB_opc_unchanged_after_disabled_cycles] >>
+    Cases_on `~enable_stg 5 (agp32 fext fbits i)` >-
+     gs [agp32_Rel_ag32_command_correct_WB_disable_fext_ready] >>
+    `(fext i).mem = (fext (m - 1 + SUC i)).mem` by fs [] >>
+    `m - 1 + SUC i = t` by fs [] >> fs [] >>
+    Cases_on `~is_wrMEM_isa (FUNPOW Next (THE (I' (5,t)) - 1) a)` >-
+     (fs [is_wrMEM_isa_def] >>
+      `(agp32 fext fbits t).WB.WB_opc <> 2w /\ (agp32 fext fbits t).WB.WB_opc <> 3w`
+        by fs [Rel_def,WB_Rel_def] >>
+      `(agp32 fext fbits (SUC i)).WB.WB_opc <> 2w /\ (agp32 fext fbits (SUC i)).WB.WB_opc <> 3w`
+        by fs [agp32_WB_opc_unchanged_when_WB_disabled] >>
+      `(agp32 fext fbits i).MEM.MEM_opc <> 2w /\ (agp32 fext fbits i).MEM.MEM_opc <> 3w`
+        by METIS_TAC [agp32_WB_opc_MEM_opc_when_WB_enabled] >> 
+      METIS_TAC [agp32_Rel_ag32_command_not_3_not_write_mem_and_byte_WB_enable]) >>
+    fs [is_wrMEM_isa_def] >-
+     (`(agp32 fext fbits (SUC t)).WB.WB_opc = 2w`
+        by fs [agp32_WB_opc_unchanged_when_WB_disabled,Rel_def,WB_Rel_def] >>
+      `(agp32 fext fbits (SUC i)).data_addr = (agp32 fext fbits (SUC t)).data_addr /\
+      (agp32 fext fbits (SUC i)).data_wdata = (agp32 fext fbits (SUC t)).data_wdata /\
+      (agp32 fext fbits (SUC i)).data_wstrb = (agp32 fext fbits (SUC t)).data_wstrb`
+        by METIS_TAC [data_addr_wdata_wstrb_unchanged_after_disabled_cycles] >>
+      `align_addr (agp32 fext fbits (SUC i)).data_addr =
+      mem_data_addr (FUNPOW Next (THE (I' (5,t)) − 1) a)`
+        by METIS_TAC [agp32_Rel_ag32_data_addr_correct_write_mem] >>
+      `(agp32 fext fbits (SUC t)).data_wdata =
+      mem_data_wdata (FUNPOW Next (THE (I' (5,t)) − 1) a)`
+        by METIS_TAC [agp32_Rel_ag32_data_wdata_correct_write_mem] >>
+      `(agp32 fext fbits (SUC t)).data_wstrb =
+      mem_data_wstrb (FUNPOW Next (THE (I' (5,t)) − 1) a)`
+        by METIS_TAC [agp32_Rel_ag32_data_wstrb_correct_write_mem] >>
+      Cases_on `THE (I' (5,t))` >-
+       METIS_TAC [WB_instr_index_not_0] >>
+      fs [FUNPOW_SUC] >>
+      qpat_abbrev_tac `ai = FUNPOW Next _ a` >>
+      fs [ag32_StoreMEM_mem_update,Rel_def]) >>
+    `(agp32 fext fbits (SUC t)).WB.WB_opc = 3w`
+      by fs [agp32_WB_opc_unchanged_when_WB_disabled,Rel_def,WB_Rel_def] >>
+    `(agp32 fext fbits (SUC i)).data_addr = (agp32 fext fbits (SUC t)).data_addr /\
+    (agp32 fext fbits (SUC i)).data_wdata = (agp32 fext fbits (SUC t)).data_wdata /\
+    (agp32 fext fbits (SUC i)).data_wstrb = (agp32 fext fbits (SUC t)).data_wstrb`
+      by METIS_TAC [data_addr_wdata_wstrb_unchanged_after_disabled_cycles] >>
+    `(agp32 fext fbits (SUC i)).data_addr = mem_data_addr (FUNPOW Next (THE (I' (5,t)) − 1) a)`
+      by METIS_TAC [agp32_Rel_ag32_data_addr_correct_write_mem_byte] >> 
+    `(agp32 fext fbits (SUC i)).data_wstrb = mem_data_wstrb (FUNPOW Next (THE (I' (5,t)) − 1) a)`
+      by METIS_TAC [agp32_Rel_ag32_data_wstrb_correct_write_mem_byte] >>
+    `word_bit 0 (mem_data_wstrb (FUNPOW Next (THE (I' (5,t)) − 1) a)) ==>
+    (7 >< 0) (agp32 fext fbits (SUC i)).data_wdata =
+    mem_data_wdata_byte (FUNPOW Next (THE (I' (5,t)) − 1) a)`
+      by METIS_TAC [agp32_Rel_ag32_data_wdata_correct_write_mem_byte_word_bit_0] >>
+    `word_bit 1 (mem_data_wstrb (FUNPOW Next (THE (I' (5,t)) − 1) a)) ==>
+    (15 >< 8) (agp32 fext fbits (SUC i)).data_wdata =
+    mem_data_wdata_byte (FUNPOW Next (THE (I' (5,t)) − 1) a)`
+      by METIS_TAC [agp32_Rel_ag32_data_wdata_correct_write_mem_byte_word_bit_1] >>
+    `word_bit 2 (mem_data_wstrb (FUNPOW Next (THE (I' (5,t)) − 1) a)) ==>
+    (23 >< 16) (agp32 fext fbits (SUC i)).data_wdata =
+    mem_data_wdata_byte (FUNPOW Next (THE (I' (5,t)) − 1) a)`
+      by METIS_TAC [agp32_Rel_ag32_data_wdata_correct_write_mem_byte_word_bit_2] >>
+    `word_bit 3 (mem_data_wstrb (FUNPOW Next (THE (I' (5,t)) − 1) a)) ==>
+    (31 >< 24) (agp32 fext fbits (SUC i)).data_wdata =
+    mem_data_wdata_byte (FUNPOW Next (THE (I' (5,t)) − 1) a)`
+      by METIS_TAC [agp32_Rel_ag32_data_wdata_correct_write_mem_byte_word_bit_3] >>
+    Cases_on `THE (I' (5,t))` >-
+     METIS_TAC [WB_instr_index_not_0] >>
+    fs [FUNPOW_SUC] >>
+    qpat_abbrev_tac `ai = FUNPOW Next _ a` >>
+    fs [Rel_def] >> METIS_TAC [ag32_StoreMEMByte_mem_update]) >-
+   (last_assum (mp_tac o is_mem_data_read `SUC i`) >> simp [] >> strip_tac >>
+    `m + SUC i = SUC t` by METIS_TAC [same_t_and_m_under_MAX_SET_SUC] >> fs [] >>
+    `I' (5,SUC t) = I' (5,t)` by fs [is_sch_def,is_sch_disable_def] >>
+    `(agp32 fext fbits (SUC i)).WB.WB_opc = (agp32 fext fbits (SUC t)).WB.WB_opc`
+      by METIS_TAC [WB_opc_unchanged_after_disabled_cycles] >>
+    Cases_on `~enable_stg 5 (agp32 fext fbits i)` >-
+     gs [agp32_Rel_ag32_command_correct_WB_disable_fext_ready] >>
+    `(fext i).mem = (fext (m - 1 + SUC i)).mem` by fs [] >>
+    `m - 1 + SUC i = t` by fs [] >> fs [] >>
+    Cases_on `~is_wrMEM_isa (FUNPOW Next (THE (I' (5,t)) - 1) a)` >-
+     fs [GSYM MEM_not_changed_after_normal_instrs,Rel_def] >>
+    fs [is_wrMEM_isa_def] >>
+    `(agp32 fext fbits (SUC t)).WB.WB_opc = (agp32 fext fbits t).WB.WB_opc`
+      by fs [agp32_WB_opc_unchanged_when_WB_disabled] >>
+    fs [Rel_def,WB_Rel_def] >>
+    gs [agp32_Rel_ag32_command_correct_write_mem_WB_enable,
+        agp32_Rel_ag32_command_correct_write_mem_byte_WB_enable]) >-
+   (last_assum (mp_tac o is_mem_inst_read `SUC i`) >> simp [] >> strip_tac >>
+    `m + SUC i = SUC t` by METIS_TAC [same_t_and_m_under_MAX_SET_SUC] >> fs [] >>
+    `I' (5,SUC t) = I' (5,t)` by fs [is_sch_def,is_sch_disable_def] >>
+    `(agp32 fext fbits (SUC i)).WB.WB_opc = (agp32 fext fbits (SUC t)).WB.WB_opc`
+      by METIS_TAC [WB_opc_unchanged_after_disabled_cycles] >>
+    Cases_on `~enable_stg 5 (agp32 fext fbits i)` >-
+     gs [agp32_Rel_ag32_command_correct_WB_disable_fext_ready] >>
+    `(fext i).mem = (fext (m - 1 + SUC i)).mem` by fs [] >>
+    `m - 1 + SUC i = t` by fs [] >> fs [] >>
+    Cases_on `~is_wrMEM_isa (FUNPOW Next (THE (I' (5,t)) - 1) a)` >-
+     fs [GSYM MEM_not_changed_after_normal_instrs,Rel_def] >>
+    fs [is_wrMEM_isa_def] >>
+    `(agp32 fext fbits (SUC t)).WB.WB_opc = (agp32 fext fbits t).WB.WB_opc`
+      by fs [agp32_WB_opc_unchanged_when_WB_disabled] >>
+    fs [Rel_def,WB_Rel_def] >>
+    gs [agp32_Rel_ag32_command_correct_write_mem_WB_enable,
+        agp32_Rel_ag32_command_correct_write_mem_byte_WB_enable]) >>
+  last_assum (mp_tac o is_mem_do_nothing `SUC i`) >> simp [] >> strip_tac >>
+  Cases_on `SUC i = t` >> fs [] >>
+  Cases_on `SUC i > t` >> fs [] >>
+  `SUC i < t` by fs [] >>
+  `(SUC i) IN {t0 | t0 < t /\ (fext t0).ready}` by fs [] >>
+  `(SUC i) <= i` by METIS_TAC [MAX_SET_DEF] >> fs []
+QED
+
+(** WB disabled **)
+Theorem agp32_Rel_ag32_fext_MEM_correct_WB_not_NONE_WB_disable:
+  !fext fbits a t I.
+    is_mem fext_accessor_circuit (agp32 fext fbits) fext ==>
+    is_sch I (agp32 fext fbits) a ==>
+    Rel I (fext t) (agp32 fext fbits (t-1)) (agp32 fext fbits t) a t ==>
+    I (5,SUC t) <> NONE ==>
+    (fext (SUC t)).ready ==>
+    ~enable_stg 5 (agp32 fext fbits t) ==>
+    (fext (SUC t)).mem = (FUNPOW Next (THE (I (5,SUC t))) a).MEM
+Proof
+  rw [] >> Cases_on `(fext t).ready` >-
+   (`I' (5,SUC t) = I' (5,t)` by fs [is_sch_def,is_sch_disable_def] >>
+    `(agp32 fext fbits (SUC t)).WB.WB_opc <> 16w` by METIS_TAC [WB_instr_index_not_NONE_opc_not_16] >>
+    `(agp32 fext fbits (SUC t)).WB.WB_opc = (agp32 fext fbits t).WB.WB_opc`
+      by fs [agp32_WB_opc_unchanged_when_WB_disabled] >>
+    last_assum (assume_tac o is_mem_def_mem_no_errors) >>
+    `(agp32 fext fbits (SUC t)).command = 0w`
+      by gs [agp32_Rel_ag32_command_correct_WB_disable_fext_ready] >>
+    last_assum (mp_tac o is_mem_do_nothing `SUC t`) >> rw [] >>
+    fs [Rel_def]) >>
+  METIS_TAC [agp32_Rel_ag32_fext_MEM_correct_WB_not_NONE_WB_disable_fext_not_ready]
 QED
 
 Theorem agp32_Rel_ag32_fext_MEM_correct_WB_not_NONE:
@@ -103,7 +451,7 @@ Theorem agp32_Rel_ag32_fext_MEM_correct_WB_not_NONE:
 Proof
   rw [] >> Cases_on `enable_stg 5 (agp32 fext fbits t)` >-
    METIS_TAC [agp32_Rel_ag32_fext_MEM_correct_WB_not_NONE_WB_enable] >>
-  cheat
+  METIS_TAC [agp32_Rel_ag32_fext_MEM_correct_WB_not_NONE_WB_disable]
 QED
 
 
@@ -143,73 +491,6 @@ Proof
 QED
 
 (** WB is disabled and fext is not ready at the previous cycle **)
-(** lemma **)
-Theorem WB_opc_unchanged_after_disabled_cycles[local]:
-  !fext fbits m n.
-    (!p. p < m ==> ~(fext (p + n)).ready) ==>
-    (agp32 fext fbits (m + n)).WB.WB_opc = (agp32 fext fbits n).WB.WB_opc
-Proof
-  rw [] >> Induct_on `m` >> rw [] >>
-  `!p. p < m ==> ~(fext (n + p)).ready` by fs [] >> fs [] >>
-  `m < SUC m` by rw [] >>
-  `~(fext (n + m)).ready` by fs [] >>
-  `~(agp32 fext fbits (n + m)).WB.WB_state_flag`
-    by METIS_TAC [agp32_WB_state_flag_and_fext_ready] >>
-  `(agp32 fext fbits (SUC (n + m))).WB.WB_opc = (agp32 fext fbits (n + m)).WB.WB_opc`
-    by fs [agp32_WB_opc_unchanged_when_WB_disabled,enable_stg_def] >>
-  `n + SUC m = SUC (n + m)` by rw [] >> rw [] >> fs []
-QED
-
-Theorem data_addr_unchanged_after_disabled_cycles[local]:
-  !fext fbits m n.
-    (!p. p < m ==> ~(fext (p + n)).ready) ==>
-    (agp32 fext fbits (m + n)).data_addr = (agp32 fext fbits n).data_addr
-Proof
-  rw [] >> Induct_on `m` >> rw [] >>
-  `!p. p < m ==> ~(fext (n + p)).ready` by fs [] >> fs [] >>
-  `m < SUC m` by rw [] >>
-  `~(fext (n + m)).ready` by fs [] >>
-  `~(agp32 fext fbits (n + m)).WB.WB_state_flag`
-    by METIS_TAC [agp32_WB_state_flag_and_fext_ready] >>
-  `(agp32 fext fbits (SUC (n + m))).data_addr = (agp32 fext fbits (n + m)).data_addr`
-    by fs [agp32_data_addr_wstrb_wdata_unchanged_when_WB_disabled,enable_stg_def] >>
-  `n + SUC m = SUC (n + m)` by rw [] >> rw [] >> fs []
-QED
-
-Theorem WB_opc_unchanged_after_disabled_cycles_0[local]:
-  !fext fbits m.
-    (!p. p < m ==> ~(fext p).ready) ==>
-    (agp32 fext fbits m).WB.WB_opc = (agp32 fext fbits 0).WB.WB_opc
-Proof
-  rw [] >> `!p. p < m ==> ~(fext (p + 0)).ready` by fs [] >>
-  `(agp32 fext fbits (m + 0)).WB.WB_opc = (agp32 fext fbits 0).WB.WB_opc`
-    by fs [WB_opc_unchanged_after_disabled_cycles] >> fs []
-QED
-
-Theorem EMPTY_no_fext_ready_cycle[local]:
-  !t fext.
-    {t0 | t0 < t /\ (fext t0).ready} = {} ==>
-    (!t0. t0 < t ==> ~(fext t0).ready)
-Proof
-  rw [] >> Cases_on `(fext t0).ready` >> rw [] >>
-  `t0 IN {t0 | t0 < t /\ (fext t0).ready}` by fs [] >>
-  METIS_TAC [MEMBER_NOT_EMPTY]
-QED
-
-Theorem MAX_SET_0_no_fext_ready_cycle[local]:
-  !t fext.
-    {t0 | t0 < t /\ (fext t0).ready} <> {} ==>
-    MAX_SET {t0 | t0 < t /\ (fext t0).ready} = 0 ==>
-    (!t0. t0 < t - 1 ==> ~(fext (t0 + 1)).ready)
-Proof
-  rw [] >>
-  `FINITE {t0 | t0 < t /\ (fext t0).ready}` by rw [FINITE_max_ready_cycle] >>
-  Cases_on `(fext (t0 + 1)).ready` >> rw [] >>
-  `t0 + 1  < t` by fs [] >>
-  `t0 + 1 IN {t0 | t0 < t /\ (fext t0).ready}` by fs [] >>
-  `t0 + 1 <= 0` by METIS_TAC [MAX_SET_DEF] >> rw []
-QED
-
 Theorem agp32_Rel_ag32_read_mem_data_rdata_correct_WB_disable_fext_not_ready:
   !fext fbits a t I.
     is_mem fext_accessor_circuit (agp32 fext fbits) fext ==>
@@ -271,7 +552,7 @@ Proof
     `opc (FUNPOW Next (THE (I' (5,t)) - 1) a) = 4w` by fs [Rel_def,WB_Rel_def] >>
     simp [mem_data_rdata_def] >>
     `(agp32 fext fbits (SUC i)).data_addr = (agp32 fext fbits (m + SUC i)).data_addr`
-      by METIS_TAC [data_addr_unchanged_after_disabled_cycles] >>
+      by METIS_TAC [data_addr_wdata_wstrb_unchanged_after_disabled_cycles] >>
     `align_addr (agp32 fext fbits (SUC t)).data_addr =
     mem_data_addr (FUNPOW Next (THE (I' (5,SUC t)) - 1) a)`
       by METIS_TAC [agp32_Rel_ag32_data_addr_correct_read_mem] >>
@@ -434,7 +715,7 @@ Proof
     `opc (FUNPOW Next (THE (I' (5,t)) - 1) a) = 5w` by fs [Rel_def,WB_Rel_def] >>
     simp [mem_data_rdata_extra_def] >>
     `(agp32 fext fbits (SUC i)).data_addr = (agp32 fext fbits (m + SUC i)).data_addr`
-      by METIS_TAC [data_addr_unchanged_after_disabled_cycles] >>
+      by METIS_TAC [data_addr_wdata_wstrb_unchanged_after_disabled_cycles] >>
     `(agp32 fext fbits (SUC i)).data_addr =
     mem_data_addr (FUNPOW Next (THE (I' (5,SUC t)) - 1) a)`
       by METIS_TAC [agp32_Rel_ag32_data_addr_correct_read_mem_byte] >> fs [] >>
